refactor

LET/proof.v
@@ -1,13 +1,10 @@
 Require Import Bool ZArith Arith List.
-Require Import Var Map.
+Require Import String.
 Set Implicit Arguments.
 
-Notation "x <- e1 ; e2" :=
-  (match e1 with
-   | Some x => e2
-   | None => None
-   end)
-    (right associativity, at level 60).
+Definition var := string.
+Definition var_eq : forall x y : var, {x = y} + {x <> y} := string_dec.
+Infix "==v" := var_eq (no associativity, at level 50).
 
 Module LetSpec.
   Inductive expression : Set :=
@@ -18,164 +15,244 @@ Module LetSpec.
   | ExpVar : var -> expression
   | ExpLet : var -> expression -> expression -> expression.
 
+  Implicit Type exp : expression.
+
   Inductive expval : Set :=
   | ValNum : Z -> expval
   | ValBool : bool -> expval.
 
-  Inductive value_of_rel : expression -> fmap var expval -> expval -> Prop :=
-  | VrelConst :
-      forall n env,
-        value_of_rel (ExpConst n) env (ValNum (Z.of_nat n))
-  | VrelDiff :
-      forall exp1 exp2 n1 n2 env,
-        value_of_rel exp1 env (ValNum n1) ->
-        value_of_rel exp2 env (ValNum n2) ->
-        value_of_rel (ExpDiff exp1 exp2) env (ValNum (n1 - n2))
-  | VrelIsZero :
-      forall exp1 n1 env,
-        value_of_rel exp1 env (ValNum n1) ->
-        value_of_rel (ExpIsZero exp1) env (ValBool (Z.eqb n1 0))
-  | VrelIfTrue :
-      forall exp1 exp2 exp3 val2 env,
-        value_of_rel exp1 env (ValBool true) ->
-        value_of_rel exp2 env val2 ->
-        value_of_rel (ExpIf exp1 exp2 exp3) env val2
-  | VrelIfFalse :
-      forall exp1 exp2 exp3 val3 env,
-        value_of_rel exp1 env (ValBool false) ->
-        value_of_rel exp3 env val3 ->
-        value_of_rel (ExpIf exp1 exp2 exp3) env val3
-  | VrelVar :
-      forall var env val,
-        env $? var = Some val -> value_of_rel (ExpVar var) env val
-  | VrelLet :
-      forall var exp1 body env val1 valb,
-        value_of_rel exp1 env val1 ->
-        value_of_rel body (env $+ (var, val1)) valb ->
-        value_of_rel (ExpLet var exp1 body) env valb.
+  Inductive environment : Set :=
+  | EnvEmpty : environment
+  | EnvExtend : var -> expval -> environment -> environment.
 
-  Hint Constructors expression expval value_of_rel.
+  Inductive behavior : Set :=
+  | BehVal : expval -> behavior
+  | BehErr : behavior.
+
+  Coercion BehVal : expval >-> behavior.
+
+  Definition empty_env := EnvEmpty.
+  Definition extend_env (env : environment) (x : var) (v : expval) := EnvExtend x v env.
+  Fixpoint apply_env (env : environment) (x : var) : behavior :=
+    match env with
+    | EnvEmpty => BehErr
+    | EnvExtend x' v env' => if x' ==v x then v else apply_env env' x
+    end.
+
+  Inductive term : Set :=
+  | TmExp : expression -> term
+  | TmDiff1 : behavior -> expression -> term
+  | TmDiff2 : expval -> behavior -> term
+  | TmIsZero1 : behavior -> term
+  | TmIf1 : behavior -> expression -> expression -> term
+  | TmLet1 : var -> behavior -> expression -> term.
+
+  Coercion TmExp : expression >-> term.
+
+  Inductive abort : behavior -> Prop :=
+  | AbrErr : abort BehErr.
+
+  Inductive is_num : expval -> Prop :=
+  | IsNum : forall n, is_num (ValNum n).
+
+  Inductive is_bool : expval -> Prop :=
+  | IsBool : forall b, is_bool (ValBool b).
+
+  Inductive value_of_rel : environment -> term -> behavior -> Prop :=
+  | VrelConst :
+      forall env n,
+        value_of_rel env (ExpConst n) (BehVal (ValNum (Z.of_nat n)))
+  | VrelDiff :
+      forall env exp1 beh1 exp2 beh,
+        value_of_rel env exp1 beh1 ->
+        value_of_rel env (TmDiff1 beh1 exp2) beh ->
+        value_of_rel env (ExpDiff exp1 exp2) beh
+  | VrefDiff1_abort :
+      forall beh1 env exp2,
+        abort beh1 ->
+        value_of_rel env (TmDiff1 beh1 exp2) beh1
+  | VrelDiff1 :
+      forall env exp2 beh2 val1 beh,
+        value_of_rel env exp2 beh2 ->
+        value_of_rel env (TmDiff2 val1 beh2) beh ->
+        value_of_rel env (TmDiff1 val1 exp2) beh
+  | VrelDiff2_abort :
+      forall beh2 env val1,
+        abort beh2 ->
+        value_of_rel env (TmDiff2 val1 beh2) beh2
+  | VrelDiff2 :
+      forall env n1 n2,
+        value_of_rel env (TmDiff2 (ValNum n1) (ValNum n2)) (ValNum (n1 - n2))
+  | VrelDiff2_err :
+      forall val1 val2 env,
+        ~(is_num val1 /\ is_num val2) ->
+        value_of_rel env (TmDiff2 val1 val2) BehErr
+  | VrelIsZero :
+      forall env exp1 beh1 beh,
+        value_of_rel env exp1 beh1 ->
+        value_of_rel env (TmIsZero1 beh1) beh ->
+        value_of_rel env (ExpIsZero exp1) beh
+  | VrelIsZero1_abort :
+      forall beh1 env,
+        abort beh1 ->
+        value_of_rel env (TmIsZero1 beh1) beh1
+  | VrelIsZero1 :
+      forall env n1,
+        value_of_rel env (TmIsZero1 (ValNum n1)) (ValBool (Z.eqb n1 0))
+  | VrelIsZero1_err :
+      forall val1 env,
+        ~is_num val1 ->
+        value_of_rel env (TmIsZero1 val1) BehErr
+  | VrelIf :
+      forall env exp1 beh1 exp2 exp3 beh,
+        value_of_rel env exp1 beh1 ->
+        value_of_rel env (TmIf1 beh1 exp2 exp3) beh ->
+        value_of_rel env (ExpIf exp1 exp2 exp3) beh
+  | VrelIf1_abort :
+      forall beh1 env exp2 exp3,
+        abort beh1 ->
+        value_of_rel env (TmIf1 beh1 exp2 exp3) beh1
+  | VrelIf1_true :
+      forall env exp2 beh2 exp3,
+        value_of_rel env exp2 beh2 ->
+        value_of_rel env (TmIf1 (ValBool true) exp2 exp3) beh2
+  | VrelIf1_false :
+      forall env exp3 beh3 exp2,
+        value_of_rel env exp3 beh3 ->
+        value_of_rel env (TmIf1 (ValBool false) exp2 exp3) beh3
+  | VrelIf1_err :
+      forall val1 env exp2 exp3,
+        ~is_bool val1 ->
+        value_of_rel env (TmIf1 val1 exp2 exp3) BehErr
+  | VrelVar :
+      forall env x,
+        value_of_rel env (ExpVar x) (apply_env env x)
+  | VrelLet :
+      forall env exp1 beh1 x exp2 beh,
+        value_of_rel env exp1 beh1 ->
+        value_of_rel env (TmLet1 x beh1 exp2) beh ->
+        value_of_rel env (ExpLet x exp1 exp2) beh
+  | VrelLet1_abort :
+      forall beh1 env x exp2,
+        abort beh1 ->
+        value_of_rel env (TmLet1 x beh1 exp2) beh1
+  | VrelLet1 :
+      forall env x val1 exp2 beh2,
+        value_of_rel (extend_env env x val1) exp2 beh2 ->
+        value_of_rel env (TmLet1 x val1 exp2) beh2.
+
+  Hint Constructors expression expval environment behavior term abort is_num is_bool value_of_rel.
 End LetSpec.
 
 Module LetImpl.
   Export LetSpec.
 
-  Inductive environment : Set :=
-  | Empty : environment
-  | Extend : var -> expval -> environment -> environment.
+  Implicit Type exp : expression.
 
-  Hint Constructors environment.
+  Notation "x <- e1 ; e2" :=
+    (match e1 with
+     | BehVal x => e2
+     | BehErr => BehErr
+     end)
+      (right associativity, at level 60).
 
-  Definition empty_env : environment := Empty.
-
-  Fixpoint apply_env (env : environment) x :=
-    match env with
-    | Empty => None
-    | Extend x' v env' => if x ==v x' then Some v else apply_env env' x
-    end.
-
-  Definition extend_env (x : var) (v : expval) (env : environment) := Extend x v env.
-
-  Definition implemented env m := forall x, apply_env env x = m $? x.
-
-  Theorem implemented_empty : implemented empty_env $0.
-    unfold implemented, empty_env, apply_env.
-    intros.
-    autorewrite with core.
-    auto.
-  Qed.
-
-  Hint Resolve implemented_empty.
-
-  Theorem implemented_extend :
-    forall env m x v,
-      implemented env m ->
-      implemented (extend_env x v env) (m $+ (x, v)).
-  Proof.
-    unfold implemented, extend_env, apply_env.
-    intros.
-    destruct (x0 ==v x); autorewrite with core; auto.
-  Qed.
-
-  Hint Resolve implemented_extend.
-
-  Function value_of (exp : expression) (env : environment) : option expval :=
+  Function value_of (env : environment) (exp : expression) : behavior :=
     match exp with
-    | ExpConst n => Some (ValNum (Z.of_nat n))
+    | ExpConst n => ValNum (Z.of_nat n)
     | ExpDiff exp1 exp2 =>
-      val1 <- value_of exp1 env;
-        val2 <- value_of exp2 env;
+      val1 <- value_of env exp1;
+        val2 <- value_of env exp2;
         match (val1, val2) with
-        | (ValNum n1, ValNum n2) => Some (ValNum (n1 - n2))
-        | _ => None
+        | (ValNum n1, ValNum n2) => ValNum (n1 - n2)
+        | _ => BehErr
         end
     | ExpIsZero exp1 =>
-      val1 <- value_of exp1 env;
+      val1 <- value_of env exp1;
         match val1 with
-        | ValNum n1 => Some (ValBool (Z.eqb n1 0))
-        | _ => None
+        | ValNum n1 => ValBool (Z.eqb n1 0)
+        | _ => BehErr
         end
     | ExpIf exp1 exp2 exp3 =>
-      val1 <- value_of exp1 env;
+      val1 <- value_of env exp1;
         match val1 with
-        | ValBool true => value_of exp2 env
-        | ValBool false => value_of exp3 env
-        | _ => None
+        | ValBool true => value_of env exp2
+        | ValBool false => value_of env exp3
+        | _ => BehErr
         end
     | ExpVar var => apply_env env var
     | ExpLet var exp1 body =>
-      val1 <- value_of exp1 env;
-        value_of body (extend_env var val1 env)
+      val1 <- value_of env exp1;
+        value_of (extend_env env var val1) body
     end.
 
+  Hint Extern 3 => match goal with
+                  | [ H : is_num (ValBool _) |- _ ] => inversion H
+                  | [ H : is_bool (ValNum _) |- _ ] => inversion H
+                  | [ |- context[is_num (ValBool _)] ] => intuition
+                  | [ |- context[is_bool (ValNum _)] ] => intuition
+                  | [ H : ~ _ |- _ ] => contradict H
+                  end.
+
   Theorem value_of_soundness :
-    forall exp env val,
-      value_of exp env = Some val ->
-      forall m,
-      implemented env m ->
-      value_of_rel exp m val.
+    forall env exp beh,
+      value_of env exp = beh ->
+      value_of_rel env exp beh.
   Proof.
-    induction exp; intros; rewrite value_of_equation in *;
-      repeat match goal with
-             | [ _ : context[match value_of ?EXP ?ENV with Some _ => _ | None => _ end] |- _ ] =>
-               destruct (value_of EXP ENV) eqn:?; try congruence
-             | [ _ : context[if ?B then _ else _] |- _ ] =>
-               destruct B
-             | [ _ : context[match ?VAL with ValNum _ => _ | ValBool _ => _ end] |- _ ] =>
+    intros env exp.
+    generalize dependent env.
+    induction exp; intros; rewrite value_of_equation in *; subst;
+      repeat
+        (try match goal with
+             | [ |- context[match value_of ?ENV ?EXP with BehVal _ => _ | BehErr => _ end] ] =>
+               destruct (value_of ENV EXP) eqn:?; try congruence
+             | [ |- context[match ?VAL with ValNum _ => _ | ValBool _ => _ end] ] =>
                destruct VAL; try congruence
-             | [ H : Some _ = Some _ |- _ ] =>
-               inversion H; clear H; subst
-             | [ H : implemented _ _ |- _ ] =>
-               unfold implemented in H; rewrite H in *
+             | [ |- context[if ?B then _ else _] ] =>
+               destruct B
              end;
-      eauto.
+         eauto 10).
   Qed.
-  
+
+  Ltac invert' H := inversion H; clear H; subst.
+
   Theorem value_of_completeness :
-    forall exp m val,
-      value_of_rel exp m val ->
-      forall env,
-      implemented env m ->
-      value_of exp env = Some val.
+    forall env exp beh,
+      value_of_rel env exp beh ->
+      value_of env exp = beh.
   Proof.
-    induction 1; intros; rewrite value_of_equation;
-      repeat match goal with
-             | [ H : forall _, implemented _ _ -> value_of _ _ = _ |- _ ] =>
-               rewrite H; clear H; subst; eauto
-             | [ H : implemented _ _ |- _ ] =>
-               unfold implemented in H; rewrite H in *
-             end;
-      eauto.
+    intros env exp.
+    generalize dependent env.
+    induction exp; intros; rewrite value_of_equation; inversion H; clear H; subst; eauto;
+    repeat
+      (try match goal with
+           | [ H : value_of_rel _ (TmDiff1 _ _) _ |- _ ] =>
+             invert' H
+           | [ H : value_of_rel _ (TmDiff2 _ _) _ |- _ ] =>
+             invert' H
+           | [ H : value_of_rel _ (TmIsZero1 _) _ |- _ ] =>
+             invert' H
+           | [ H : value_of_rel _ (TmIf1 _ _ _) _ |- _ ] =>
+             invert' H
+           | [ H : value_of_rel _ (TmLet1 _ _ _) _ |- _ ] =>
+             invert' H
+           | [ IH : forall _ _, value_of_rel _ ?EXP _ -> _, H : value_of_rel _ ?EXP _ |- _ ] =>
+             apply IH in H; rewrite H
+           | [ H : abort _ |- _ ] =>
+             invert' H
+           | [ |- context[match ?VAL with ValNum _ => _ | ValBool _ => _ end] ] =>
+             destruct VAL; try congruence
+           end;
+       eauto 10).
   Qed.
 
   Hint Resolve value_of_soundness value_of_completeness.
   
   Theorem value_of_correctness :
-    forall exp val,
-      value_of exp empty_env = Some val <->
-      value_of_rel exp $0 val.
+    forall exp beh,
+      value_of empty_env exp = beh <->
+      value_of_rel empty_env exp beh.
   Proof.
-    split; eauto.
+    intuition.
   Qed.
 End LetImpl.
 
